dafny/engine.dfy
@@ -1,0 +1,65 @@
+/**
+  * Core Execution Engine
+  */
+
+include "./token.dfy"
+include "./state.dfy"
+include "./process.dfy"
+include "./utils/variables.dfy"
+module ExecutionEngine {
+  import opened Token
+  import opened BPMNState
+  import opened ProcessDefinition
+  import opened Variables
+
+  /**
+    * The main execution function
+    */
+  function ExecuteStep(state: State): State
+    requires state.Running?
+    requires ValidState(state)
+    ensures ValidState(ExecuteStep(state))
+  {
+    var process := state.process;
+    var activeTokens := GetActiveTokens(process.tokenCollection);
+
+    if |activeTokens| == 0 then
+      Completed(process, process.globalVariables)
+    else
+      var tokenId := Token.PickOne(activeTokens);
+      ExecuteTokenStep(state, tokenId)
+  }
+
+  /**
+    * Execute the step of a single token
+    */
+  function ExecuteTokenStep(state: State, tokenId: Token.TokenId): State
+    requires state.Running?
+    requires tokenId in GetActiveTokens(state.process.tokenCollection)
+    requires tokenId in state.process.tokenCollection.tokens
+    requires state.process.tokenCollection.tokens[tokenId].location in state.process.processDefinition.nodes
+  {
+    var process := state.process;
+    var token := process.tokenCollection.tokens[tokenId];
+    var currentNode := process.processDefinition.nodes[token.location];
+
+    match currentNode.nodeType {
+      case StartEvent => ExecuteStartEvent(state, tokenId)
+      case EndEvent => ExecuteEndEvent(state, tokenId)
+      case Task(taskType) => ExecuteTask(state, tokenId, taskType)
+      case Gateway(gatewayType) => ExecuteGateway(state, tokenId, gatewayType)
+      case IntermediateEvent(eventType) => ExecuteIntermediateEvent(state, tokenId, eventType)
+    }
+  }
+
+  // execute the step of a start event
+  function ExecuteStartEvent(state: State, tokenId: Token.TokenId): State { state }
+  // execute the step of a end event
+  function ExecuteEndEvent(state: State, tokenId: Token.TokenId): State { state }
+  // execute the step of a task
+  function ExecuteTask(state: State, tokenId: Token.TokenId, taskType: TaskType): State { state }
+  // execute the step of a gateway
+  function ExecuteGateway(state: State, tokenId: Token.TokenId, gatewayType: GatewayType): State { state }
+  // execute the step of a intermediate event
+  function ExecuteIntermediateEvent(state: State, tokenId: Token.TokenId, eventType: ProcessDefinition.EventType): State { state }
+} 
