dafny/process.dfy
@@ -1,0 +1,68 @@
+/**
+  * Process Definition Module
+  * 
+  */
+include "utils/option.dfy"
+module ProcessDefinition {
+  import opened Optional
+
+  /**
+    * Node Type
+    */
+  datatype NodeType =
+    | StartEvent
+    | EndEvent
+    | Task(taskType: TaskType)
+    | Gateway(gatewayType: GatewayType)
+    | IntermediateEvent(eventType: EventType)
+
+  /**
+    * Task Type
+    */
+  datatype TaskType =
+    | UserTask
+    | ServiceTask
+    | ScriptTask
+    | BusinessRuleTask
+
+
+  datatype GatewayType =
+    | ExclusiveGateway
+    | ParallelGateway
+    | InclusiveGateway
+    | EventBasedGateway
+
+
+  datatype EventType =
+    | MessageEvent
+    | TimerEvent
+    | SignalEvent
+    | ErrorEvent
+
+
+  datatype Node = ProcessNode(
+    id: string,
+    name: string,
+    nodeType: NodeType,
+    incoming: set<string>,
+    outgoing: set<string>
+  )
+
+
+  datatype SequenceFlow = Flow(
+    id: string,
+    sourceRef: string,
+    targetRef: string,
+    condition: Option<string>
+  )
+
+
+  datatype ProcessDef = ProcessDefinition(
+    id: string,
+    name: string,
+    nodes: map<string, Node>,
+    flows: map<string, SequenceFlow>,
+    startNodes: set<string>,
+    endNodes: set<string>
+  )
+} 
