dafny/utils/variables.dfy
@@ -1,0 +1,43 @@
+/**
+  * BPMN 变量管理模块
+  */
+include "option.dfy"
+module Variables {
+  import opened Optional
+
+  /**
+    * 变量值类型
+    */
+  datatype VariableValue =
+    | StringValue(stringValue: string)
+    | IntValue(intValue: int)
+    | BoolValue(boolValue: bool)
+    | ListValue(values: seq<VariableValue>)
+    | ObjectValue(fields: map<string, VariableValue>)
+
+  /**
+    * 变量映射
+    */
+  type VariableMap = map<string, VariableValue>
+
+  /**
+    * 创建空变量映射
+    */
+  function EmptyVariables(): VariableMap {
+    map[]
+  }
+
+  /**
+    * 设置变量值
+    */
+  function SetVariable(vars: VariableMap, name: string, value: VariableValue): VariableMap {
+    vars[name := value]
+  }
+
+  /**
+    * 获取变量值
+    */
+  function GetVariable(vars: VariableMap, name: string): Option<VariableValue> {
+    if name in vars then Some(vars[name]) else None
+  }
+}
